<?xml version="1.0" encoding="UTF-8"?>

<section xml:id="sec-2.2-ops-on-sets" xmlns:xi="http://www.w3.org/2001/XInclude">
  <title>Operations on Sets</title>
  
  <p> 
    If the set <m>A</m> contains all the elements that the set <m>B</m> does, we call <m>B</m> a <em>subset</em>
    of <m>A</m>. Conversely, we call <m>A</m> a <em>superset</em> of <m>B</m>. 
  </p>
  <definition xml:id="def-Subset-and-Superset">
    <!-- there was some notes on <notation> and <usage> tags in here; review
      later -->
      <notation>
        <usage><m>\subseteq, \subset</m></usage>
        <description><m>B</m> is a <m>\subseteq</m> of <m>A</m></description>
      </notation>
    <statement>
      <p>
        <term>Subset &amp; Superset.</term> The set <m>B</m> is a <term>subset</term> of the set <m>A</m>, written <m>B \subseteq A</m>, if for all
        <m>b \in B</m> we also have <m>b \in A</m>.
        In this case, <m>A</m> is called a <term>superset</term> of <m>B</m>.
        <fn>
          Some mathematicians use the symbol <m>\subset</m> instead of <m>\subseteq</m>.
        </fn>
      </p>
    </statement>
  </definition>

  <p>
    More text here...
  </p>

  <definition xml:id="def-">
    <notation>
      <usage><m>=</m></usage>
      <description></description>
    </notation>
    <statement>
      <p> 
        <term>Set Equality</term>. The sets <m>A</m> and <m>B</m> are <term>equal</term>,
        written <m>A = B</m>, if <m>A \subseteq B</m> and <m>B \subseteq A</m>
        
      </p>
    </statement>
  </definition>

  <p>
    Having a definition of equality to lean on will help us when we need to prove things about sets.
  </p>

  <example>
    <title>Proving Set Equality</title>
      <statement>
        <p>
          Let <m>A</m> be the set of numbers that can be expressed
          as <m>2n</m> for some whole number <m>n</m>, and let <m>B</m> be the
          set of numbers that can be expressed as <m>m + 1</m> where <m>m</m> is
          an odd whole number.  We will show <m>A = B</m>.
        </p>
        
        <p>
          First, let us show <m>A \subseteq B</m>.  If <m>x \in A</m>, then <m>x = 2n</m>
          for some whole number <m>n</m>.  Therefore 
          <me>
            x=2n=2(n-1)+1+1=m+1
          </me> 
          
          where
          <m>m=2(n-1)+1</m> is, by definition, an odd number.  Thus <m>x \in B</m>,
          which proves <m>A \subseteq B</m>.
        </p>
        
        <p>
          Now we will show <m>B \subseteq A</m>.  Let <m>x \in A</m>.  By definition,
          <m>x=m+1</m> for some odd <m>m</m>. By the definition of oddness, <m>m=2k+1</m>
          for some whole number <m>k</m>. Thus
          <md>
            <mrow>x=m+1\amp=(2k+1)+1=2k+2</mrow>
            <mrow> \amp =2(k+1)=2n,</mrow>
          </md>

          where <m>n=k+1</m>, and so <m>x\in A</m>.  Since <m>A\subseteq B</m>
	        and <m>B\subseteq A</m>, by definition <m>A=B</m>.
        </p>

      </statement>
    
  </example>

</section>